Test/dafny0/ByMethodResolution.dfy
@@ -89,3 +89,69 @@ module ByMethodGhostInterests {
     rr := G(x, true);
   }
 }
+
+module BadExtremeRecursion {
+  // P and F are not allowed in the same recursive cluster
+  least predicate P() {
+    F() == 5 // error: this call is illegal
+  }
+  function F(): int {
+    if P() then 5 else 3
+  } by method {
+    return 5;
+  }
+
+  // no problem with Q and G
+  least predicate Q() {
+    G() == 5
+  }
+  function G(): int {
+    5
+  } by method {
+    ghost var u := Q();
+    return 5;
+  }
+
+  // no problem with R0/H0'/H0
+  least predicate R0() {
+    H0'() == 5
+  }
+  function H0'(): int {
+    if H0() < 100 then 5 else 3 // in a ghost context, this calls the function part of H0
+  }
+  function H0(): int {
+    5
+  } by method {
+    var x := H0'();
+    var y := R0();
+    return 5;
+  }
+
+  // R1/H1'/H1 are mutually recursive
+  least predicate R1() {
+    H1'() == 5 // error: R1 is in same recursive cluster as H1
+  }
+  function method H1'(): int {
+    if H1() < 100 then 5 else 3 // in a compiled context, this calls the method part of H1
+  }
+  function H1(): int {
+    5
+  } by method {
+    var x :=  H1'();
+    var y := R1();
+    return 5;
+  }
+
+  // R2/H2'/H2 are mutually recursive
+  least predicate R2() {
+    H2'() == 5 // error: R2 is in same recursive cluster as H2
+  }
+  function method H2'(): int {
+    if H2() < 100 then 5 else 3 // in a compiled context, this calls the method part of H2
+  }
+  function H2(): int {
+    if R2() then 5 else 3
+  } by method { // the method part uses the function part in its specification, so there's a call-graph edge
+    return 5;
+  }
+}
